pattenrs for FuncView
- removing whitespace.

theories/Views/FuncView.v
@@ -1,26 +1,73 @@
 Require Import ExtLib.Data.Map.FMapPositive.
 Require Import ExtLib.Data.SumN.
 Require Import ExtLib.Data.Positive.
+Require Import MirrorCore.Views.Ptrns.
 
 Set Implicit Arguments.
 Set Strict Implicit.
 Set Maximal Implicit Insertion.
 
-Class FuncView (func A : Type) := {
-  f_insert : A -> func;
-  f_view : func -> option A
-}.
+Section FuncView.
+  Variables func A : Type.
 
-Class FuncViewOk (func A : Type) (FV : FuncView func A) := {
-  fv_ok : forall f a, f_view f = Some a <-> f_insert a = f
-}.                                               
+  Class FuncView : Type :=
+  { f_insert : A -> func
+  ; f_view : func -> option A
+  }.
+
+  Variable FV : FuncView.
+
+  Class FuncViewOk : Type :=
+  { fv_ok : forall f a, f_view f = Some a <-> f_insert a = f
+  }.
+
+  Definition ptrn_view {T} (p : ptrn A T) : ptrn func T :=
+    fun e _T good bad =>
+      match f_view e with
+      | None => bad e
+      | Some f => p f _T good (fun _ => bad e)
+      end.
+
+  Theorem ptrn_view_ok T (p : ptrn A T) : ptrn_ok p -> ptrn_ok (ptrn_view p).
+  Proof.
+    unfold ptrn_view, ptrn_ok, Succeeds, Fails.
+    intros.
+    destruct (f_view x).
+    { specialize (H a).
+      destruct H.
+      { left. destruct H. exists x0.
+        setoid_rewrite H. reflexivity. }
+      { right. setoid_rewrite H. reflexivity. } }
+    { eauto. }
+  Qed.
+
+  Variable FVO : FuncViewOk.
+
+  Theorem Succeeds_ptrn_view {T} (p : ptrn A T) x res (H : ptrn_ok p)
+  : Succeeds x (ptrn_view p) res ->
+    exists f, f_insert f = x /\ Succeeds f p res.
+  Proof.
+    unfold Succeeds, ptrn_view. intros.
+    destruct (f_view x) eqn:Heq.
+    { eapply fv_ok in Heq.
+      eexists; split; eauto.
+      destruct (H a).
+      { destruct H1. red in H1. setoid_rewrite H1 in H0.
+        setoid_rewrite H1. eauto. }
+      { red in H1. setoid_rewrite H1 in H0.
+        specialize (H0 _ (fun _ => true) (fun _ => false)); inversion H0. } }
+    { exfalso.
+      specialize (H0 _ (fun _ => true) (fun _ => false)); inversion H0. }
+  Qed.
+End FuncView.
+
 
 Section FuncViewSumN.
   Context {A func : Type}.
 
-  Global Instance FuncViewPMap (p : positive) (m : FMapPositive.pmap Type) 
+  Global Instance FuncViewPMap (p : positive) (m : FMapPositive.pmap Type)
 	 (pf : Some A = pmap_lookup' m p) :
-    FuncView (OneOf m) A := 
+    FuncView (OneOf m) A :=
     {
       f_insert f := Into f p pf;
       f_view f :=
@@ -28,10 +75,10 @@ Section FuncViewSumN.
 	  | Build_OneOf _ p' pf1 =>
 	    match Pos.eq_dec p p' with
 	      | left Heq =>
-	       Some (eq_rect_r (fun o => match o with 
-                                           | Some T => T 
+	       Some (eq_rect_r (fun o => match o with
+                                           | Some T => T
                                            | None => Empty_set
-                                         end) pf1 
+                                         end) pf1
 	                       (eq_rect _ (fun p => Some A = pmap_lookup' m p) pf _ Heq))
 	      | right _ => None
 	    end
@@ -39,7 +86,7 @@ Section FuncViewSumN.
 
     }.
 
-  Global Instance FuncViewOkPMap (p : positive) (m : FMapPositive.pmap Type) 
+  Global Instance FuncViewOkPMap (p : positive) (m : FMapPositive.pmap Type)
 	 (pf : Some A = pmap_lookup' m p) :
     FuncViewOk (FuncViewPMap p m pf) := _.
   Proof.
